1) Convertir la coordenada $(6,\frac{\pi}{3},\frac{\pi}{6})$ esférica al sistema rectangular.

\[x = \rho cos \theta sin \varphi = 6 \cdot cos \left(\frac{\pi}{3}\right) \cdot sin \left( \frac{\pi}{6} \right) = \frac{3}{2}\]
\[y = \rho sin \theta sin \varphi = 6 \cdot sin \left( \frac{\pi}{3} \right) \cdot sin \left(\frac{\pi}{6} \right) =\frac{3\sqrt{3}}{2}\]
\[z = \rho cos \varphi = 6 \cdot cos \left(\frac{\pi}{6} \right) = 3 \sqrt{3}\]

\vspace{4mm}
2) Convertir la coordenada $(0, \pi , \frac{\pi}{5})$ esférica al sistema rectangular.

\[x = \rho cos \theta sin \varphi = 0 \cdot cos (\pi) \cdot sin \left(\frac{\pi}{5}\right) = 0\]
\[y = \rho sin \theta sin \varphi = 0 \cdot sin \left(\pi \right) \cdot sin \left(\frac{\pi}{5} \right) = 0\]
\[z = \rho cos \varphi = 0 \cdot cos \left(\frac{\pi}{5} \right) = 0\]

\vspace{4mm}
3) Convertir la coordenada $\left( 3, 0, \frac{\pi}{3} \right)$ esférica al sistema rectangular.

\[x = \rho cos \theta sin \varphi = 3 \cdot cos\left( 0\right) \cdot sin \left(\frac{\pi}{3}\right) = 3 \cdot (1) \left(\frac{\sqrt{3}}{2} \right) = \frac{3\sqrt{3}}{2}\]
\[y = \rho sin \theta sin \varphi = 3 \cdot sin(0) \cdot sin \left( \frac{\pi}{3} \right) = 3 \cdot (0) \cdot \left(\frac{\sqrt{3}}{2}\right) = 0  \]
\[z = \rho cos \varphi = 3 \cdot cos \left( \frac{\pi}{3}\right) = 3 \cdot \left(\frac{1}{2}\right) =\frac{3}{2}\]

\vspace{4mm}
4) Convertir la coordenada $\left(3, \frac{\pi}{3},0\right)$ esférica al sistema rectangular.

\[x = \rho cos \theta sin \varphi = 3 \cdot sin \left(\frac{\pi}{3}\right) \cdot sin (0) =  3 \cdot \left(\frac{1}{2}\right) \cdot (0) = 0 \]
\[y = \rho sin \theta sin \varphi = 3 \cdot sin \left(\frac{\pi}{3}\right) sin (0) = 3 \cdot \left(\frac{\sqrt{3}}{2}\right) \cdot (0) = 0\]
\[z = \rho cos \varphi = 3 \cdot cos(0) = 3(1) = 3we
 \]
